cellio/CellioAll.v
@@ -5,62 +5,67 @@ From CRIS.cellio Require Import CellioHeader CellioA CellioI MainA MainI CellioI
 Section CellioAux.
   Context `{!crisG Γ Σ α β τ Hsub Hinv, _CELL: !cellioGS}.
 
-  Variable CtxA : SMod.t.
-  Hypothesis ctx_real: SMod.is_real CtxA.
-  Hypothesis ctx_mod_wf: Mod.wf (SMod.to_mod ∅ CtxA).
-  Hypothesis ctx_cancellable : SMod.cancellable CtxA.
-  Hypothesis ctx_has_input: fid CtxHdr.input ∈ dom (SMod.fnsems CtxA).
-  Hypothesis ctx_has_foo: fid CtxHdr.foo ∈ dom (SMod.fnsems CtxA).
+  Variable Ctx : SMod.t.
+  Hypothesis ctx_real: SMod.is_real Ctx.
+  Hypothesis ctx_mod_wf: Mod.wf (SMod.to_mod ∅ Ctx).
+  Hypothesis ctx_cancellable : SMod.cancellable Ctx.
+  Hypothesis ctx_has_input: fid CtxHdr.input ∈ dom (SMod.fnsems Ctx).
+  Hypothesis ctx_has_foo: fid CtxHdr.foo ∈ dom (SMod.fnsems Ctx).
   Hypothesis ctx_main_disj:
-    ∀ fno, fno ∈ dom (SMod.fnsems CtxA) → fno ∈ dom (Mod.fnsems MainI.t) → False.
+    ∀ fno, fno ∈ dom (SMod.fnsems Ctx) → fno ∈ dom (Mod.fnsems MainI.t) → False.
   Hypothesis ctx_cellio_disj:
-    ∀ fno, fno ∈ dom (SMod.fnsems CtxA) → fno ∈ dom (Mod.fnsems CellioI.t) → False.
+    ∀ fno, fno ∈ dom (SMod.fnsems Ctx) → fno ∈ dom (Mod.fnsems CellioI.t) → False.
   Hypothesis ctx_main_scope_disj:
-    ∀ mn, mn ∈ (SMod.scopes CtxA) → mn ∈ (Mod.scopes MainI.t) → False.
+    ∀ mn, mn ∈ (SMod.scopes Ctx) → mn ∈ (Mod.scopes MainI.t) → False.
   Hypothesis ctx_cellio_scope_disj:
-    ∀ mn, mn ∈ (SMod.scopes CtxA) → mn ∈ (Mod.scopes CellioI.t) → False.
+    ∀ mn, mn ∈ (SMod.scopes Ctx) → mn ∈ (Mod.scopes CellioI.t) → False.
 
-  Local Definition smod_src : SMod.t := MainA.smod ☆ CtxA.
-  Local Definition mod_top : Mod.t := SMod.to_mod ∅ (SMod.cancel smod_src).
+  Local Definition Ctx_filtered : SMod.t := SMod.filter (CFilter.msk_filter_out {[MainAS.main]}) (SMod.filter SFilter.msk_filter_out Ctx).
+  Local Definition mod_top : Mod.t := SMod.to_mod ∅ (SMod.cancel (MainA.smod ☆ Ctx_filtered)).
+  Local Definition mod_tgt : Mod.t := MainI.t ★ CellioI.t ★ SMod.to_mod ∅ Ctx.
 
-  Local Definition sp : specmap := SMod.conc_sp_from smod_src.
-  Local Definition mod_src : Mod.t := SMod.to_mod sp smod_src.
-  Local Definition mod_tgt : Mod.t := MainI.t ★ CellioI.t ★ (SMod.to_mod sp CtxA).
+  Local Definition sp : specmap := SMod.sp_from (MainA.smod ☆ Ctx_filtered).
+  Local Definition mod_src : Mod.t := SMod.to_mod sp MainA.smod ★ SMod.to_mod ∅ Ctx.
 
   Local Definition init_cond : iProp Σ :=
     (CellioA.init_cond)%I.
 
   Lemma sp_input: sp.1 !! fid CtxHdr.input = None.
   Proof.
-    rewrite /sp /SMod.conc_sp_from /= /smod_src /SMod.sp_core_from.
-    i. rewrite lookup_omap !lookup_fmap lookup_omap lookup_union_with.
-    rewrite /MainA.fnsems. simpl_map.
-    assert (FIND: exists x, SMod.fnsems CtxA !! fid CtxHdr.input = Some (Some x)).
+    rewrite lookup_omap !lookup_fmap lookup_omap lookup_union_with.
+    assert (FIND: exists x, SMod.fnsems Ctx !! fid CtxHdr.input = Some (Some x)).
     { eapply elem_of_dom in ctx_has_input. inv ctx_has_input. eauto.
       inv ctx_mod_wf. destruct x; eauto.
-      destruct (SMod.fnsems CtxA !! fid CtxHdr.input) eqn:FIND; ss.
+      destruct (SMod.fnsems Ctx !! fid CtxHdr.input) eqn:FIND; ss.
       inv H. hexploit (wf_fns (fid CtxHdr.input)).
       { rewrite /Mod.fnsems /SMod.to_mod lookup_fmap FIND //. }
       i. ss. inv H.
     }
-    des. rewrite FIND. ss. destruct x, p. r in ctx_real. hexploit ctx_real; eauto.
+    des. rewrite !lookup_fmap FIND. ss. destruct x, p. eauto.
   (*SLOW*)Qed.
 
   Lemma sp_foo: sp.1 !! fid CtxHdr.foo = None.
   Proof.
-    rewrite /sp /SMod.conc_sp_from /= /smod_src /SMod.sp_core_from.
     rewrite lookup_omap !lookup_fmap lookup_omap lookup_union_with.
-    rewrite /MainA.fnsems. simpl_map.
-    assert (FIND: exists x, SMod.fnsems CtxA !! fid CtxHdr.foo = Some (Some x)).
+    assert (FIND: exists x, SMod.fnsems Ctx !! fid CtxHdr.foo = Some (Some x)).
     { eapply elem_of_dom in ctx_has_foo. inv ctx_has_foo. eauto.
       inv ctx_mod_wf. destruct x; eauto.
-      destruct (SMod.fnsems CtxA !! fid CtxHdr.foo) eqn:FIND; ss.
+      destruct (SMod.fnsems Ctx !! fid CtxHdr.foo) eqn:FIND; ss.
       inv H. hexploit (wf_fns (fid CtxHdr.foo)).
       { rewrite /Mod.fnsems /SMod.to_mod lookup_fmap FIND //. }
       i. ss. inv H.
     }
-    des. rewrite FIND. ss. destruct x, p. r in ctx_real. hexploit ctx_real; eauto.
+    des. rewrite !lookup_fmap FIND. ss. destruct x, p. et.
   (*SLOW*)Qed.
+
+  Lemma sp_main: sp.1 !! fid MainAS.main = Some (MainAS.main_spec: fspec_rel).
+  Proof.
+    rewrite lookup_omap !lookup_fmap lookup_omap lookup_union_with. simpl_map.
+    destruct (SMod.fnsems Ctx_filtered !! fid MainAS.main) eqn: Lctxf_main; et.
+    exfalso. eapply (ctx_main_disj (fid MainAS.main)); rewrite elem_of_dom; et.
+    rewrite !lookup_fmap in Lctxf_main.
+    destruct (SMod.fnsems _ !! _) eqn: Lctx_main; ss.
+  Qed.
   
   (* Apply cancellation to linked spec module *)
   Lemma cancel_src:
@@ -68,18 +73,52 @@ Section CellioAux.
       (mod_src, init_cond)
       (mod_top, init_cond ∗ CellioA.cell 0 ∗ Cancel.init_res)%I.
   Proof.
-    etrans. { eapply ctxr_refines, Cancel.cancellation_prepare; et; clarify. }
+    etrans.
+    { eapply ctxr_refines. ctxr_drop.
+      eapply SFilter.smod_filter_intro. }
+    etrans.
+    { eapply ctxr_refines. ctxr_drop.
+      eapply CFilter.smod_filter_intro with (bl:={[MainAS.main]}). }
+    etrans.
+    { eapply ctxr_refines. ctxr_rotate. ctxr_drop.
+      eapply Cancel.cancellation_prepare; et; clarify.
+    }
+    etrans.
+    { eapply ctxr_refines. ctxr_rotate. ctxr_drop.
+      eapply Cancel.cancellation_prepare with (sps := sp); et; i; cycle 1.
+      { rewrite SFilter.cfilter_comm in H0.
+        eapply SFilter.filter_masked; et.
+      }
+      
+      ltac2:(renames H into Lfn, Lsp).
+      eapply CFilter.filter_masked; et.
+      rewrite lookup_empty in Lsp. apply not_eq_sym, not_eq_None_Some in Lsp.
+      destruct Lsp as [? Lsp]. eapply SMod.sp_core_from_add_lookup in Lsp.
+      destruct Lsp as [Lsp|Lsp]; des; cycle 1.
+      - eapply SMod.sp_core_from_lookup in Lsp0; des.
+        rewrite !lookup_fmap in Lsp0.
+        destruct (SMod.fnsems Ctx !! _) as [[[? []]|]|] eqn: Lctx_fc; ss; subst.
+        eapply ctx_real in Lctx_fc; subst; ss.
+      - eapply SMod.sp_core_from_lookup in Lsp; des.
+        rewrite lookup_insert_Some in Lsp; des; ss. 
+        rewrite lookup_singleton_Some in Lsp1. set_solver.
+    }
+
+    rewrite -SMod.to_mod_cancel_add left_id.
     eapply Cancel.cancellation.
-    { apply SMod.cancellable_add; r; rewrite /= /MainA.fnsems //; mod_tac ss. }
-    { assert (Ce : SMod.fnsems CtxA !! entry = None).
+    { apply SMod.cancellable_add.
+      - r; rewrite /= /MainA.fnsems //; mod_tac ss.
+      - eapply CFilter.filter_cancellable, SFilter.filter_cancellable. et.
+    }
+    { assert (Ce : SMod.fnsems Ctx !! entry = None).
       { eapply not_elem_of_dom. ii. eapply ctx_main_disj; eauto.
         rewrite /MainI.t /MainI.smod /SMod.to_mod /= /Mod.fnsems. set_solver.
       }
-      assert (Ht : (SMod.conc_sp_from smod_src).1 !! entry =
+      assert (Ht : (SMod.sp_from (MainA.smod ☆ Ctx_filtered)).1 !! entry =
         fsp_some MainAS.main_spec); last (rewrite Ht; clear Ht).
-      { rewrite /SMod.conc_sp_from /SMod.sp_core_from.
+      { rewrite /SMod.sp_from /SMod.sp_core_from.
         rewrite !lookup_omap !lookup_fmap lookup_omap lookup_union_with.
-        simpl_map; ss. rewrite Ce //.
+        simpl_map; ss. rewrite !lookup_fmap Ce //.
       }
       eexists _, _; splits.
       { ss; exists tt; split; refl. }
@@ -92,8 +131,7 @@ Section CellioAux.
   Lemma src_tgt : refines (mod_tgt, emp%I) (mod_src, init_cond)%I.
   Proof.
     eapply ctxr_refines.
-    rewrite /init_cond /mod_src /smod_src /mod_tgt.
-    rewrite !SMod.to_mod_add.
+    rewrite /init_cond /mod_src /mod_tgt.
     
     (* solve by transitivity:
       MainI ★ CellioI ⊆ MainI ★ CellioA ⊆ MainA ★ CellioA 
@@ -107,11 +145,11 @@ Section CellioAux.
     etrans.
     { (* MainI ★ CellioA ⊆ MainA *)
       ctxr_rotate. ctxr_drop. ctxr_rotate.
-      eapply main_adequacy, MainIA.sim; eauto using sp_input, sp_foo.
+      eapply main_adequacy, MainIA.sim; eauto using sp_input, sp_foo, sp_main.
     }
 
     etrans.
-    { (* CtxA ⊆ CtxA *)
+    { (* Ctx ⊆ Ctx *)
       ctxr_rotate. ctxr_drop. refl.
     }
     
@@ -136,7 +174,7 @@ Section CellioAux.
     { eapply Mod.add_wf.
       { econs; eauto; [mod_tac|prove_nodup]. }
       { inv ctx_mod_wf. econs.
-        { ii. destruct (SMod.fnsems CtxA !! i) eqn: FIND.
+        { ii. destruct (SMod.fnsems Ctx !! i) eqn: FIND.
           { rewrite /Mod.fnsems /SMod.to_mod lookup_fmap FIND /= in H. inv H.
             destruct o; ss. hexploit (wf_fns i); eauto.
             rewrite /Mod.fnsems /SMod.to_mod lookup_fmap FIND //.
@@ -176,24 +214,24 @@ Module CellioAll.
 
   Lemma behavioral_refinement :
     ∃ β τ (Hinv : invGS Γ Σ α) (_ : crisG Γ Σ α β τ _ Hinv) (_ : cellioGS),
-    ∀ (CtxA : SMod.t)
-      (ctx_real: SMod.is_real CtxA)
-      (ctx_mod_wf: Mod.wf (SMod.to_mod ∅ CtxA))
-      (ctx_cancellable : SMod.cancellable CtxA)
-      (ctx_has_input: fid CtxHdr.input ∈ dom (SMod.fnsems CtxA))
-      (ctx_has_foo: fid CtxHdr.foo ∈ dom (SMod.fnsems CtxA))
+    ∀ (Ctx : SMod.t)
+      (ctx_real: SMod.is_real Ctx)
+      (ctx_mod_wf: Mod.wf (SMod.to_mod ∅ Ctx))
+      (ctx_cancellable : SMod.cancellable Ctx)
+      (ctx_has_input: fid CtxHdr.input ∈ dom (SMod.fnsems Ctx))
+      (ctx_has_foo: fid CtxHdr.foo ∈ dom (SMod.fnsems Ctx))
       (ctx_main_disj:
-        ∀ fno, fno ∈ dom (SMod.fnsems CtxA) → fno ∈ dom (Mod.fnsems MainI.t) → False)
+        ∀ fno, fno ∈ dom (SMod.fnsems Ctx) → fno ∈ dom (Mod.fnsems MainI.t) → False)
       (ctx_cellio_disj:
-        ∀ fno, fno ∈ dom (SMod.fnsems CtxA) → fno ∈ dom (Mod.fnsems CellioI.t) → False)
+        ∀ fno, fno ∈ dom (SMod.fnsems Ctx) → fno ∈ dom (Mod.fnsems CellioI.t) → False)
       (ctx_main_scope_disj:
-        ∀ mn, mn ∈ (SMod.scopes CtxA) → mn ∈ (Mod.scopes MainI.t) → False)
+        ∀ mn, mn ∈ (SMod.scopes Ctx) → mn ∈ (Mod.scopes MainI.t) → False)
       (ctx_cellio_scope_disj:
-        ∀ mn, mn ∈ (SMod.scopes CtxA) → mn ∈ (Mod.scopes CellioI.t) → False),
+        ∀ mn, mn ∈ (SMod.scopes Ctx) → mn ∈ (Mod.scopes CellioI.t) → False),
     ∃ src_res tgt_res,
     refines_lmod
-      (Mod.to_lmod (mod_tgt CtxA) tgt_res)
-      (Mod.to_lmod (mod_top CtxA) src_res).
+      (Mod.to_lmod (mod_tgt Ctx) tgt_res)
+      (Mod.to_lmod (mod_top Ctx) src_res).
   Proof.
     apply own_admin_soundness.
     iMod cris_alloc as "[% [% [% [% ?]]]]".
