celliocb/CelliocbAll.v
@@ -7,56 +7,53 @@ Require Import
 Section CelliocbAux.
   Context `{!crisG Γ Σ α β τ Hsub Hinv, _CELL: !celliocbGS}.
 
-  Variable CtxcbI : SMod.t.
-  Hypothesis ctx_real: SMod.is_real CtxcbI.
-  Hypothesis ctx_mod_wf: Mod.wf (SMod.to_mod ∅ CtxcbI).
-  Hypothesis ctx_cancellable : SMod.cancellable CtxcbI.
-  Hypothesis ctx_has_foo: fid CtxcbHdr.foo ∈ dom (SMod.fnsems CtxcbI).
+  Variable Ctx : SMod.t.
+  Hypothesis ctx_real: SMod.is_real Ctx.
+  Hypothesis ctx_mod_wf: Mod.wf (SMod.to_mod ∅ Ctx).
+  Hypothesis ctx_cancellable : SMod.cancellable Ctx.
+  Hypothesis ctx_has_foo: fid CtxcbHdr.foo ∈ dom (SMod.fnsems Ctx).
   Hypothesis ctx_main_disj:
-    ∀ fno, fno ∈ dom (SMod.fnsems CtxcbI) → fno ∈ dom (Mod.fnsems MaincbI.t) → False.
+    ∀ fno, fno ∈ dom (SMod.fnsems Ctx) → fno ∈ dom (Mod.fnsems MaincbI.t) → False.
   Hypothesis ctx_cellio_disj:
-    ∀ fno, fno ∈ dom (SMod.fnsems CtxcbI) → fno ∈ dom (Mod.fnsems CelliocbI.t) → False.
+    ∀ fno, fno ∈ dom (SMod.fnsems Ctx) → fno ∈ dom (Mod.fnsems CelliocbI.t) → False.
   Hypothesis ctx_main_scope_disj:
-    ∀ mn, mn ∈ (SMod.scopes CtxcbI) → mn ∈ (Mod.scopes MaincbI.t) → False.
+    ∀ mn, mn ∈ (SMod.scopes Ctx) → mn ∈ (Mod.scopes MaincbI.t) → False.
   Hypothesis ctx_cellio_scope_disj:
-    ∀ mn, mn ∈ (SMod.scopes CtxcbI) → mn ∈ (Mod.scopes CelliocbI.t) → False.
+    ∀ mn, mn ∈ (SMod.scopes Ctx) → mn ∈ (Mod.scopes CelliocbI.t) → False.
 
-  Local Definition smod_src : SMod.t := MaincbA.smod ☆ CtxcbI.
-  Local Definition mod_top : Mod.t := SMod.to_mod ∅ (SMod.cancel smod_src).
+  Local Definition Ctx_filtered : SMod.t := SMod.filter SFilter.msk_filter_out Ctx.
+  Local Definition mod_top : Mod.t := SMod.to_mod ∅ (SMod.cancel (MaincbA.smod ☆ Ctx_filtered)).
+  Local Definition mod_tgt : Mod.t := MaincbI.t ★ CelliocbI.t ★ (SMod.to_mod ∅ Ctx).
 
-  Local Definition sp : specmap := SMod.conc_sp_from smod_src.
-  Local Definition mod_src : Mod.t := SMod.to_mod sp smod_src.
-  Local Definition mod_tgt : Mod.t := MaincbI.t ★ CelliocbI.t ★ (SMod.to_mod sp CtxcbI).
+  Local Definition sp : specmap := SMod.sp_from (MaincbA.smod ☆ Ctx_filtered).
+  Local Definition mod_src : Mod.t := SMod.to_mod sp MaincbA.smod ★ SMod.to_mod ∅ Ctx.
 
   Local Definition init_cond : iProp Σ :=
     (CelliocbA.init_cond)%I.
 
+  Lemma sp_cb: sp.1 !! fid MaincbHdr.input_cb = None.
+  Proof.
+    rewrite lookup_omap !lookup_fmap lookup_omap lookup_union_with.
+    assert (CTXNONE: SMod.fnsems Ctx !! fid MaincbHdr.input_cb = None).
+    { eapply not_elem_of_dom. ii. eapply ctx_main_disj; eauto.
+      rewrite /MaincbI.t /MaincbI.smod /SMod.to_mod /= /Mod.fnsems. set_solver.
+    } 
+    des. rewrite !lookup_fmap CTXNONE. ss.
+  (*SLOW*)Qed.
+
   Lemma sp_foo: sp.1 !! fid CtxcbHdr.foo = None.
   Proof.
-    rewrite /sp /SMod.conc_sp_from /= /smod_src /SMod.sp_core_from.
     rewrite lookup_omap !lookup_fmap lookup_omap lookup_union_with.
-    assert (FIND: exists x, SMod.fnsems CtxcbI !! fid CtxcbHdr.foo = Some (Some x)).
+    assert (FIND: exists x, SMod.fnsems Ctx !! fid CtxcbHdr.foo = Some (Some x)).
     { eapply elem_of_dom in ctx_has_foo. inv ctx_has_foo. eauto.
       inv ctx_mod_wf. destruct x; eauto.
-      destruct (SMod.fnsems CtxcbI !! fid CtxcbHdr.foo) eqn:FIND; ss.
+      destruct (SMod.fnsems Ctx !! fid CtxcbHdr.foo) eqn:FIND; ss.
       inv H. hexploit (wf_fns (fid CtxcbHdr.foo)).
       { rewrite /Mod.fnsems /SMod.to_mod lookup_fmap FIND //. }
       i. ss. inv H.
     }
-    des. rewrite FIND. ss. destruct x, p. r in ctx_real. hexploit ctx_real; eauto.
+    des. rewrite !lookup_fmap FIND. ss. destruct x, p. et.
   (*SLOW*)Qed.
-
-  Lemma sp_cb: sp.1 !! fid MaincbHdr.input_cb = None.
-  Proof.
-    rewrite /sp /SMod.conc_sp_from /= /smod_src /SMod.sp_core_from.
-    rewrite lookup_omap !lookup_fmap lookup_omap lookup_union_with.
-    assert (CTXNONE: SMod.fnsems CtxcbI !! fid MaincbHdr.input_cb = None).
-    { eapply not_elem_of_dom. ii. eapply ctx_main_disj; eauto.
-      rewrite /MaincbI.t /MaincbI.smod /SMod.to_mod /= /Mod.fnsems. set_solver.
-    } 
-    des. rewrite CTXNONE. ss.
-  (*SLOW*)Qed.
-
 
   (* Apply cancellation to linked spec module *)
   Lemma cancel_src:
@@ -64,18 +61,46 @@ Section CelliocbAux.
       (mod_src, init_cond)
       (mod_top, init_cond ∗ CelliocbA.cell 0 ∗ Cancel.init_res)%I.
   Proof.
-    etrans. { eapply ctxr_refines, Cancel.cancellation_prepare; et; clarify. }
+    etrans.
+    { eapply ctxr_refines. ctxr_drop.
+      eapply SFilter.smod_filter_intro. }
+    etrans.
+    { eapply ctxr_refines. ctxr_rotate. ctxr_drop.
+      eapply Cancel.cancellation_prepare; et; clarify.
+    }
+
+    etrans.
+    { eapply ctxr_refines. ctxr_rotate. ctxr_drop.
+      eapply Cancel.cancellation_prepare with (sps:=sp); et; i; cycle 1.
+      { eapply SFilter.filter_masked; et. }
+
+      ltac2:(renames H into Lfn, Lsp).
+      rewrite lookup_empty in Lsp. apply not_eq_sym, not_eq_None_Some in Lsp.
+      destruct Lsp as [? Lsp]. eapply SMod.sp_core_from_add_lookup in Lsp.
+      destruct Lsp as [Lsp|Lsp]; des; cycle 1.
+      - eapply SMod.sp_core_from_lookup in Lsp0; des. rewrite !lookup_fmap in Lsp0.
+        destruct (SMod.fnsems Ctx !! _) as [[[? []]|]|] eqn: Lctx_fc; ss; subst.
+        eapply ctx_real in Lctx_fc; subst; ss.
+      - eapply SMod.sp_core_from_lookup in Lsp; des.
+        rewrite lookup_insert_Some in Lsp; des; ss. 
+        rewrite lookup_singleton_Some in Lsp1. set_solver.
+    }
+
+    rewrite -SMod.to_mod_cancel_add left_id.
     eapply Cancel.cancellation.
-    { apply SMod.cancellable_add; r; rewrite /= /MaincbA.fnsems //; mod_tac ss. }
-    { assert (Ce : SMod.fnsems CtxcbI !! entry = None).
+    { apply SMod.cancellable_add.
+      - r; rewrite /= /MaincbA.fnsems //; mod_tac ss.
+      - eapply SFilter.filter_cancellable. et.
+    }
+    { assert (Ce : SMod.fnsems Ctx !! entry = None).
       { eapply not_elem_of_dom. ii. eapply ctx_main_disj; eauto.
         rewrite /MaincbI.t /MaincbI.smod /SMod.to_mod /= /Mod.fnsems. set_solver.
       }
-      assert (Ht : (SMod.conc_sp_from smod_src).1 !! entry =
+      assert (Ht : (SMod.sp_from (MaincbA.smod ☆ Ctx_filtered)).1 !! entry =
         fsp_some MaincbA.main_spec); last (rewrite Ht; clear Ht).
-      { rewrite /SMod.conc_sp_from /SMod.sp_core_from.
+      { rewrite /SMod.sp_from /SMod.sp_core_from.
         rewrite !lookup_omap !lookup_fmap lookup_omap lookup_union_with.
-        simpl_map; ss. rewrite Ce //.
+        simpl_map; ss. rewrite !lookup_fmap Ce //.
       }
       eexists _, _; splits.
       { ss; exists tt; split; refl. }
@@ -88,8 +113,7 @@ Section CelliocbAux.
   Lemma src_tgt : refines (mod_tgt, emp%I) (mod_src, init_cond)%I.
   Proof.
     eapply ctxr_refines.
-    rewrite /init_cond /mod_src /smod_src /mod_tgt.
-    rewrite !SMod.to_mod_add.
+    rewrite /init_cond /mod_src /mod_tgt.
     
     (* solve by transitivity:
       MaincbI ★ CelliocbI ⊆ MaincbI ★ CelliocbA ⊆ MaincbA ★ CelliocbA 
@@ -107,7 +131,7 @@ Section CelliocbAux.
     }
 
     etrans.
-    { (* CtxcbI ⊆ CtxcbI *)
+    { (* Ctx ⊆ Ctx *)
       ctxr_rotate. ctxr_drop. refl.
     }
 
@@ -132,7 +156,7 @@ Section CelliocbAux.
     { eapply Mod.add_wf.
       { econs; eauto; [mod_tac|prove_nodup]. }
       { inv ctx_mod_wf. econs.
-        { ii. destruct (SMod.fnsems CtxcbI !! i) eqn: FIND.
+        { ii. destruct (SMod.fnsems Ctx !! i) eqn: FIND.
           { rewrite /Mod.fnsems /SMod.to_mod lookup_fmap FIND /= in H. inv H.
             destruct o; ss. hexploit (wf_fns i); eauto.
             rewrite /Mod.fnsems /SMod.to_mod lookup_fmap FIND //.
@@ -172,23 +196,23 @@ Module CelliocbAll.
 
   Lemma behavioral_refinement :
     ∃ β τ (Hinv : invGS Γ Σ α) (_ : crisG Γ Σ α β τ _ Hinv) (_ : celliocbGS),
-    ∀ (CtxcbI : SMod.t)
-      (ctx_real: SMod.is_real CtxcbI)
-      (ctx_mod_wf: Mod.wf (SMod.to_mod ∅ CtxcbI))
-      (ctx_cancellable : SMod.cancellable CtxcbI)
-      (ctx_has_foo: fid CtxcbHdr.foo ∈ dom (SMod.fnsems CtxcbI))
+    ∀ (Ctx : SMod.t)
+      (ctx_real: SMod.is_real Ctx)
+      (ctx_mod_wf: Mod.wf (SMod.to_mod ∅ Ctx))
+      (ctx_cancellable : SMod.cancellable Ctx)
+      (ctx_has_foo: fid CtxcbHdr.foo ∈ dom (SMod.fnsems Ctx))
       (ctx_main_disj:
-        ∀ fno, fno ∈ dom (SMod.fnsems CtxcbI) → fno ∈ dom (Mod.fnsems MaincbI.t) → False)
+        ∀ fno, fno ∈ dom (SMod.fnsems Ctx) → fno ∈ dom (Mod.fnsems MaincbI.t) → False)
       (ctx_cellio_disj:
-        ∀ fno, fno ∈ dom (SMod.fnsems CtxcbI) → fno ∈ dom (Mod.fnsems CelliocbI.t) → False)
+        ∀ fno, fno ∈ dom (SMod.fnsems Ctx) → fno ∈ dom (Mod.fnsems CelliocbI.t) → False)
       (ctx_main_scope_disj:
-        ∀ mn, mn ∈ (SMod.scopes CtxcbI) → mn ∈ (Mod.scopes MaincbI.t) → False)
+        ∀ mn, mn ∈ (SMod.scopes Ctx) → mn ∈ (Mod.scopes MaincbI.t) → False)
       (ctx_cellio_scope_disj:
-        ∀ mn, mn ∈ (SMod.scopes CtxcbI) → mn ∈ (Mod.scopes CelliocbI.t) → False),
+        ∀ mn, mn ∈ (SMod.scopes Ctx) → mn ∈ (Mod.scopes CelliocbI.t) → False),
     ∃ src_res tgt_res,
     refines_lmod
-      (Mod.to_lmod (mod_tgt CtxcbI) tgt_res)
-      (Mod.to_lmod (mod_top CtxcbI) src_res).
+      (Mod.to_lmod (mod_tgt Ctx) tgt_res)
+      (Mod.to_lmod (mod_top Ctx) src_res).
   Proof.
     apply own_admin_soundness.
     iMod cris_alloc as "[% [% [% [% ?]]]]".
